prop lib

hax-lib/proofs/fstar/extraction/Hax_lib.fst
@@ -1,12 +1,14 @@
 module Hax_lib
+
 #set-options "--fuel 0 --ifuel 1 --z3rlimit 15"
 open FStar.Tactics
+open Hax_lib.Prop
 
-val v_assert (p: bool) : Pure unit (requires p) (ensures (fun x -> p))
-let v_assert (v__formula: bool) = ()
+val v_assert (p: t_Prop) : Pure unit (requires p) (ensures (fun x -> p))
+let v_assert (v__formula: t_Prop) = ()
 
-val v_assume (p: bool) : Pure unit (requires True) (ensures (fun x -> p))
-let v_assume (v__formula: bool) = assume v__formula
+val v_assume (p: t_Prop : Pure unit (requires True) (ensures (fun x -> p))
+let v_assume (v__formula: t_Prop) = assume v__formula
 
 
 unfold let v_exists (v__f: 'a -> t_Prop): t_Prop = exists (x: 'a). v__f x
