hax-lib/proofs/fstar/extraction/Hax_lib.Abstraction.fst
@@ -1,0 +1,1 @@
+module Hax_lib.Abstraction
