hax-lib/proofs/fstar/extraction/Hax_lib.Prop.fst
@@ -1,0 +1,3 @@
+module Hax_lib.Prop
+
+type t_Prop = Type0
